<?xml version="1.0" encoding="UTF-8"?>

<section xml:id="sec1-5-hom-system" xmlns:xi="http://www.w3.org/2001/XInclude">
  <title>Homogeneous System of Linear Equations</title>
    <p>
     <definition xml:id="def-homo-system">
        <statement>
            <p>
                A system  <m>AX = B</m> of linear equations
is called <alert> homogeneous</alert> if 
<m>B = 0</m>. Otherwise it is called a  <alert>  non homogeneous</alert>  system.
          </p>
        </statement>
     </definition>   
    </p>
<p>
    Observe that any homogeneous system <m>AX = 0</m> of linear
equations has at least one solution, namely the trivial solution (<m>x_i = 0</m>, for all <m>i</m>).  The augmented matrix is
got from adding one zero column to <m>A</m>. Hence <m>.r(A) =
r(A^*)</m>.
</p>
<theorem xml:id="thm-hom-system1">
        <statement>
        <p>
            A homogeneous system  <m>AX = 0</m> of <m>n</m> equations
            in the
            same number of unknowns (<m>n</m> unknowns) has a nontrivial
            solution if and only if <m>A</m> is singular, that is , if and
            only if <m>\det(A)=0</m>.      
        </p>
    </statement>

    <proof>
        <p>
            
        The given  homogeneous system has a nontrivial
        solution if and only if it has infinitely many solutions,
        if and only if <m>r(A)\lt n</m>, the number of variables (<xref ref="thm-nosol-rank"/>).
        But <m>r(A)\lt n </m>, if and only if <m>A</m> is singular.
        </p>
    </proof>
</theorem>

    <theorem xml:id="thm-hom-system2">
        <statement>
            <p>
                A homogeneous system  <m>AX = 0</m> of <m>m</m> equations
in <m>n</m> unknowns, where <m>m \lt n</m> has infinitely many nontrivial solutions.
            </p>
        </statement>
    
    <proof>
        If <m>m \lt n</m>, then <m>r(A) \lt  n</m> and hence the result follows from thm.~
        <xref ref="thm-nosol-rank"/>.
    </proof>

</theorem>

<p>
    We would
like to get the connection between solutions of a homogeneous system
<m>AX = 0</m> and  the solutions of <m>AX = B</m>, <m>B \neq 0</m>. These
are stated in the following Theorem.
</p>

<theorem xml:id="thm-hom-system3">
        <statement>
            <p>
                Suppose the non homogeneous system <m>AX
                = B</m> of linear equations has a solution say <m>X = X_0</m>.
                All the solutions of this system are of the form
                <me>X_0 + X_h,</me>
                where <m>X_h</m> runs through all the solutions of the
                corresponding homogeneous system <m>AX =0</m>. 
            </p>
        </statement>

        <proof>
            <p>
                Let <m>X_h</m> be a solution of <m>AX=0</m>. Then 
                <me>A(X_0 + X_h) = AX_0 + A
                    X_h = B + 0 = B</me>. Hence <m>X_0 +X_h</m> is a solution of <m>AX =
                    B</m>. 
                    </p>
                    <p>  
                    Suppose <m>Y</m> is a solution of <m>AX = B</m>, i.e. <m>AY = B</m>.
                    Then <m>A (Y - X_0) = 0</m> and hence <m>Y-X_0</m> is a solution of
                    <m>AX = 0</m> and <m>Y = X_0+(Y-X_0)=X_0+X_h</m>, where <m>X_h=Y-X_0</m>.
            </p>
        </proof>
    </theorem>

    <p> 
        The above theorem can be written equivalently as
    </p>  

        <theorem xml:id="thm-hom-system4">
            <statement>
                <p>
                    
            If <m>(\alpha_1 ,\ldots, \alpha_n)</m> is a solution of a system of linear equations, then
            the complete solution is given by <m>x_1 = \alpha_1 + y_1 ,\ldots , x_n = \alpha_n + y_n</m> , where
            <m>(y_1 ,\ldots, y_n)</m> is the general solution of the associated homogeneous system.
                </p>
            </statement>
        </theorem>
        
        
            <example>
                <p>
                Let us consider one equation in two variables, <m>2x_1+3x_2=5</m>. 
                The corresponding homogeneous system is <m>2x_1+3x_2=0</m>. It is easy see that 
                <m>\left\{\begin{pmatrix} \alpha\\-\frac{2}{3}\alpha\end{pmatrix}:\alpha\in \R\right\}</m> 
                is set of all solutions of  <m>2x_1+3x_2=0</m>. Let us consider a solution 
                <m>X_0=\begin{pmatrix} 0\\\frac{5}{3}\end{pmatrix}</m> of the non homogeneous system 
                <m>2x_1+3x_2=5</m>.  Let <m>X=\begin{pmatrix} \alpha\\-\frac{2}{3}\alpha\end{pmatrix}</m> 
                be any solution of <m>2x_1+3x_2=0</m>. Then it is easy to check that 
                <m>X_0+X=\begin{pmatrix} \alpha\\\frac{5}{3}-\frac{2}{3}\alpha\end{pmatrix}</m> 
                is a solution of <m>2x_1+3x_2=5</m>.
                
                Alternatively, to solve <m>2x_1+3x_2=5</m>, we can free one of the variable say <m>x_1</m>. That is <m>x_1</m> can take any real value. Let <m>x_1=\alpha</m>,  then <m>x_2=\frac{5}{3}-\frac{2}{3}\alpha</m>. Hence a generic solution of <m>2x_1+3x_2=5</m> is given by <m>\begin{pmatrix}x_1\\x_2\end{pmatrix}=\begin{pmatrix} \alpha\\\frac{5}{3}-\frac{2}{3}\alpha\end{pmatrix}</m>, which can be rewritten as 
                <m>
                \begin{pmatrix} \alpha\\\frac{5}{3}-\frac{2}{3}\alpha\end{pmatrix}=\begin{pmatrix} 0\\\frac{5}{3}\end{pmatrix}+\begin{pmatrix} \alpha\\-\frac{2}{3}\alpha\end{pmatrix}
                </m>. 
                Thus all solutions of <m>2x_1+3x_2=5</m> are of the form 
                <me>
                \left\{\begin{pmatrix} 0\\\frac{5}{3}\end{pmatrix}+\begin{pmatrix} \alpha\\-\frac{2}{3}\alpha\end{pmatrix} :\alpha \in \R\right\}=\left\{\begin{pmatrix} 0\\\frac{5}{3}\end{pmatrix}+\alpha\begin{pmatrix} 1\\-\frac{2}{3}\end{pmatrix} :\alpha \in \R\right\}.
                </me>
                Notice that tho two lines, <m>2x_1+3x_2=5</m> and <m>2x_1+3x_2=0</m> are parallel to each other. Plot the figure in Sage using the following Sage sybtax.
    
                <sage>
                    <input>
                    <![CDATA[    
                    var('x,y')
                    l1 = implicit_plot(2*x+3*y==5,(x,-5,5),(y,-5,5),gridlines='minor')
                    l2= implicit_plot(2*x+3*y==0,(x,-5,5),(y,-5,5),color='red',gridlines='minor')
                    p1 = point((0,5/3),color='blue',size=20)
                    p0 = point((1,-2/3),color='red',size=20)
                    t0 =text('$(1,-\\frac{-2}{3})$',(1,-1.5),color='red')
                    t1 =text('$(0,-\\frac{5}{3})$',(1,5/3),color='blue')
                    show(l1+l2+p0+p1+t0+t1,axes=True,figsize=5)
                    ]]>
                    </input>
                    <output>
                        
                    </output>
                </sage>
        
        </p>
            </example>
    
        
    
            <example>
                <p>
                Let consider 2 equations in three variables.
                <men xml:id="eqn-hom-eg1-1">2x_1-x_2-x_3=5; x_1+x_2-2x_3=7 </men>
                
                The corresponding homogeneous system is given by 
                <men xml:id="eqn-hom-eg1-2">	2x_1-x_2-x_3=0; x_1+x_2-2x_3=0	</men>.
                It is easy to see that the set of all solutions of the homogeneous system <xref ref="eqn-hom-eg1-2"/> is 
                <me>
                \begin{bmatrix} x_1\\x_2\\ x_3\end{bmatrix}=\left\{ 
                \begin{bmatrix} \alpha\\ \alpha\\ \alpha\end{bmatrix}:
                \alpha\in \R
                \right\}
                </me><xref ref="eqn-hom-eg1-1"/>, we get <m>3x_1-3x_3=12</m> which implies <m>x_1=4+x_3</m>. 
            Now substituting <m>x_1=4+x_3</m> in the second equation of <xref ref="eqn-hom-eg1-1"/>, we get <m>x_2=3+x_3</m>. 
            Here we can take <m>x_3</m> as a free variable, hence any solution of~<xref ref="eqn-hom-eg1-1"/> is of the form 
            <me>\begin{bmatrix}4+\alpha\\3+\alpha\\\alpha\end{bmatrix}</me> which can be written as <me>\begin{bmatrix}4\\3\\0\end{bmatrix}+\begin{bmatrix}\alpha\\\alpha\\\alpha\end{bmatrix}</me>. Note that <m>\begin{bmatrix}4\\3\\0\end{bmatrix}</m> is a solution <xref ref="eqn-hom-eg1-1"/>. Thus set of all solution of <xref ref="eqn-hom-eg1-1"/> is of the form 
                <me>
                \begin{bmatrix} x_1\\x_2\\ x_3\end{bmatrix}=\left\{ 
                \begin{bmatrix}4\\3\\0\end{bmatrix}+\begin{bmatrix} \alpha\\ \alpha\\ \alpha\end{bmatrix}:
                \alpha\in \R
                \right\}
                </me>
                
                <p>
                    Geometrically, each equation in the non homogeneous system represents a plane and the solution is the line of intersection of the the two planes. 

                    Similarly, each equation of the corresponding homogeneous system represents a plane passing through the origin and parallel to the corresponding plane of the non homogeneous system. Thus the solution of the corresponsing homogeneosu system in the line of intersection of the the two planes passing through the origin. Thus the solutions of the system and the corresponsing homogeneous system are parallel lines. Visualize this using the following Sage syntax.
                    
                        <sage>
                            <input>
                            <![CDATA[
                            var('x,y,z,t')
                            eq1 = 2*x-y-z-5
                            eq2 = x+y-2*z-7
                            plane1 = implicit_plot3d(eq1,(x,-5,5),(y,-5,5),(z,-5,5),opacity=0.4)
                            plane2 = implicit_plot3d(eq2,(x,-5,5),(y,-5,5),(z,-5,5),color='red',opacity=0.4)
                            l1 = parametric_plot3d([4+t,3+t,t],(t,-5,5),color='black',thikness=15)
                            plane10 = implicit_plot3d(eq1+5,(x,-5,5),(y,-5,5),(z,-5,5),opacity=0.4)
                            plane20 = implicit_plot3d(eq2+7,(x,-5,5),(y,-5,5),(z,-5,5),color='red',opacity=0.4)
                            l0 = parametric_plot3d([t,t,t],(t,-5,5),color='black',thikness=15)
                            show(plane1+plane2+l1+plane10+plane20+l0,axes=True,frame=False)
                            ]]>
                            </input>
                            <output>
                                
                            </output>
                        </sage>

                </p>
            </p>
            </example>
    
        
</section>
