<?xml version="1.0" encoding="UTF-8"?>

<section xml:id="sec3-2-LT" xmlns:xi="http://www.w3.org/2001/XInclude">
  <title>Linear maps from <m>\R^n</m> to <m>\R^m</m></title>
  <introduction>
    <p>
      In this section, we wish to find linear maps from <m>\R^n</m> to <m>\R^m</m>. We shall see that these 
      linear maps are essentially given by an <m>m\times n</m> matrix. We shall also see how to find 
      matrix of a linear transformation with respect to a given basis on domain and codomain. 
    </p>
  </introduction>

  <subsection xml:id="sec3-2-LT-RntoRm">
    <title>Linear maps from <m>\R^n</m> to <m>\R^m</m></title>
 <p>   
     We want to find a linear map from <m>\R^n</m> to <m>\R^m</m>.
    Suppose <m>T\colon \R^n\to \R^m</m> is a linear map.
    Then for <m>x\in \R^n</m>, <m>T(x)\in \R^m</m>.
    In particular, <m>T(x)</m> has <m>m</m> components.
    Let us write these components as <m>T_1(x),\ldots, T_m(x)</m>.
    Thus <m>T</m> is given by
    <me>
      T(x)=\begin{bmatrix}T_1(x)\\T_2(x)\\\vdots\\T_m(x) \end{bmatrix}
    </me>.
  </p>

  <p>
    Note that for each <m>i=1,\ldots, m</m>,
    <m>T_i</m> is a map from <m>\R^n\to \R</m>.
  </p>
  
  <exercise xml:id="linalg-engg-ex29">
    <statement>
      <p>
        Show that <m>T\colon \R^n\to \R^m</m> defined by
        <m>T(x)=\left(T_1(x),\ldots, T_m(x)\right)</m> is linear map if and only if
        <m>T_i\colon \R^n\to \R</m> is linear map for each <m>i</m>.
      </p>
    </statement>
  </exercise>

  <p>
    From Ex.
    <xref ref="linalg-engg-ex29"></xref>,
    it follows that in order to know linear map <m>T</m>,
    it is sufficient to know component <m>T_i\colon \R^n\to \R</m> for each <m>i</m>.
  </p>

  <example><title>Linear map from <m>\R^n</m> to <m>\R</m></title>
    <statement>
      <p>
        Suppose <m>T\colon \R^n\to \R</m> is a linear map.
        Consider the standard basis <m>\beta=\{e_1,e_2,\ldots,
        e_n\}</m>.
        Then for <m>x\in \R^n</m>, we have <m>x=x_1e_1+x_2e_2+\cdots+x_n e_n</m>.
        Since <m>T</m> is linear, we have
        <md>
          <mrow> T(x)=\amp T(x_1e_1+x_2e_2+\cdots+x_n e_n)</mrow>
            <mrow> =\amp x_1T(e_2)+x_2T(e_2)+\cdots+x_n T(e_n)</mrow>
        </md>.
      </p>
      <p>
        Define <m>T(e_1):=a_1, T(e_2):=a_2,\ldots, T(e_n):=a_n</m>.
        Then
        <me>
          T(x)=a_1x_1+a_2x_2+\cdots+a_nx_n
        </me>.
      </p>
  
      <p>
        Thus, if <m>T\colon \R^n\to \R</m> is a linear map,
        there there exist scalars,
        <m>a_1,a_2,\ldots,a_n</m> such that <m>T(x)=a_1x_1+a_2x_2+\cdots+a_nx_n</m>.
        Here we have <m>a_i=T(e_i)</m> for <m>i=1,\ldots,n</m>.
        It is clear that to know <m>T</m> it is good enough to know <m>T(e_1),\ldots, T(e_n)</m>.
      </p>
      <p>
        What we have proved is, any linear map <m>T</m> from 
        <m>\R^n\to \R</m> is given by 
        <me>
          T(x)=a_1x_1+a_2x_2+\cdots+a_nx_n
        </me>
         where <m>a_i=T(e_i)</m> for <m>1\leq i\leq n</m>.
      </p>

      <p>
        What happens if you chose a different basis (other than standard basis)? 
      </p>
    </statement>
  </example>

  <p>
    Let us come back to the linear map <m>T(x)=\begin{bmatrix}T_1(x)\\T_2(x)\\\vdots\\T_m(x) \end{bmatrix}</m>.
    Since for each <m>i</m>, <m>T_i</m> is linear, there exist scalars,
    <m>a_{i1},a_{i2},\ldots,a_{in}\in \R</m> such that <m>T_i(x)=a_{i1}x_1+a_{i2}x_2+\cdots+a_{i_n}x_n</m>.
    Thus
    <me>
      T(x)=\begin{bmatrix}a_{11}x_1+a_{12}x_2+\cdots+a_{1n}x_n\\ a_{21}x_1+a_{22}x_2+\cdots+a_{2n}x_n\\\vdots\\ a_{m1}x_1+a_{m2}x_2+\cdots+a_{mn}x_n \end{bmatrix} = \begin{bmatrix}a_{11}\amp a_{12}\amp \cdots\amp a_{1n}\\ a_{21}\amp a_{22}\amp \cdots\amp a_{2n}\\ \vdots \amp \vdots\amp \ddots\amp \vdots\\ a_{m1}\amp a_{m2}\amp \cdots\amp a_{mn} \end{bmatrix}  \begin{bmatrix}x_1\\x_2\\\vdots \\x_n \end{bmatrix}
    </me>.
  </p>
  
  <p>
    Thus we have shown that any linear map
    <m>T\colon \R^n\to\R^m</m> is a matrix transformation <m>T_A</m>,
    where <m>A=[a_{ij}]</m>.
    Note that the matrix of <m>T</m>
    <md>
      <mrow>A =
        \begin{bmatrix}a_{11}\amp a_{12}\amp \cdots\amp a_{1n}\\ a_{21}\amp a_{22}\amp \cdots\amp a_{2n}\\ \vdots \amp \vdots\amp \ddots\amp \vdots\\ a_{m1}\amp a_{m2}\amp \cdots\amp a_{mn} \end{bmatrix} 
        = \amp\begin{bmatrix}T_1(e_1)\amp T_1(e_2)\amp \cdots\amp T_1(e_n)\\ T_2(e_1)\amp T_2(e_2)\amp \cdots\amp T_2(e_n)\\ \vdots \amp \vdots\amp \ddots\amp \vdots\\ T_m(e_1)\amp T_m(e_2)\amp \cdots\amp T_m(e_n) \end{bmatrix} </mrow>
        <mrow>=\amp \begin{bmatrix}T(e_1)\amp T(e_2)\amp \cdots \amp  T(e_n) \end{bmatrix}</mrow>
    </md>.
  </p>
  
  <p>
    Notice that the <m>j</m>-th columns of <m>A</m> is the coordinates of the vector <m>T(e_j)</m> with respect to the standard basis <m>\{e_1,\ldots,e_m\}</m> of <m>\R^m</m>.
    Thus to find the matrix of <m>T</m>,
    we find the coordinates of <m>T(e_j)</m> with respect to the basis on the codomain and put it in the <m>j</m>-th column.
  </p>
  
  <p>
    What happens if we change the bases on <m>\R^n</m> and <m>\R^m</m>.
    In order to see this let us consider an example.
  </p>
  
  <example xml:id="ling-engg-eg31">
    <statement>
      <p>
        Consider a linear map <m>T\colon \R^3\to \R^2</m> defined by <m>T\left(\begin{bmatrix}x_1\\x_2\\x_3 \end{bmatrix} \right)=\begin{bmatrix}2x_1-x_2+x_3\\x_1+x_2-x_3 \end{bmatrix}</m>.
        It is easy to see that <m>T</m> is a matrix transformation <m>T_A</m> where <m>A=\begin{bmatrix}2 \amp -1 \amp 1\\1 \amp 1\amp -1 \end{bmatrix}</m>.
        In particular,
        <m>A</m> is the matrix of <m>T</m> when we consider standard bases on the domain <m>\R^3</m> and codomain <m>\R^2</m>.
      </p>
      <p>
        Let us consider a basis <m>\beta =\{v_1=(1,1,-1),v_2=(1,-1,1),v_3=(-1,1,1)\}</m> of the domain and the standard basis <m>\gamma=\{(1,0),(0,1)\}</m> on the codomain.
        In order to find the matrix <m>A</m> of <m>T</m>,
        we find the image of <m>T(v_1)</m> and find its coordinates with respect to the standard basis <m>\gamma</m>.
        We have <m>T(v_1)=(0,3)</m>.
        Thus the first columns of <m>A</m> is <m>\begin{bmatrix}0\\3 \end{bmatrix}</m>.
        Similarly <m>T(v_2)=(4,-1)</m> and <m>T(v_3)=(2,-1)</m>.
        Hence the matrix of <m>A</m> of <m>T</m> with respect to the basis <m>\beta</m> and <m>\gamma</m> is <m>\begin{bmatrix}0\amp 4 \amp 2\\3\amp -1\amp -1 \end{bmatrix}</m>.
        We denote this matrix as <m>[T]_\beta^\gamma</m>.
      </p>
    </statement>
  </example>

  <exercise xml:id="exer-3-2-4">
    <statement>
      <p>
        Consider the linear transformation defined in the <xref ref="ling-engg-eg31">Example</xref>.
        Find the matrix of <m>T</m> with respect to a basis
        <m>\beta =\{v_1=(1,1,-1),v_2=(1,-1,1),v_3=(-1,1,1)\}</m> of <m>\R^3</m> and <m>\gamma=\{w_2=(1,-1),(2,1)\}</m> of <m>\R^2</m>.
      </p>
    </statement>
  </exercise>

  <example xml:id="ling-engg-eg33">
    <statement>
      <p>
        Consider a linear map <m>T\colon \R^3\to \R^3</m> given by <m>T\left(\begin{bmatrix}x_1\\x_2\\x_3 \end{bmatrix} \right)=\begin{bmatrix}2x_1-x_2+x_3\\x_1+x_2-x_3\\3x_1+2x_3 \end{bmatrix}</m>.
        Let us find the matrix of <m>T</m> with respect to a basis
        <m>\beta =\{v_1=(1,1,-1),v_2=(1,-1,1),v_3=(-1,1,1)\}</m> of <m>\R^3</m> on the domain and codomain.
        Note that columns of <m>[T]_\beta^\beta</m> are the coordinates of
        <m>T(v_1), T(v_2), T(v_3)</m> with respect to the basis <m>\beta</m>.
        This can be obtained simultaneously by applying RREF to
        <m>\begin{bmatrix}v_1 \amp  v_2 \amp  v_3 \amp  T(v_1)\amp  T(v_2)\amp  T(v_3) \end{bmatrix}</m> 
        and taking the last three columns as <m>[T]_\beta^\beta</m>.
        <md>
          <mrow>\amp \begin{bmatrix}v_1 \amp  v_2 \amp  v_3 \amp  T(v_1)\amp  T(v_2)\amp  T(v_3) \end{bmatrix} </mrow>
          <mrow>   =\amp \left[\begin{array}{rrrrrr} 1 \amp  1 \amp  -1 \amp  0 \amp  4 \amp  -2 \\ 1 \amp  -1 \amp  1 \amp  3 \amp  -1 \amp  -1 \\ -1 \amp  1 \amp  1 \amp  1 \amp  5 \amp  -1 \end{array} \right]
           \xrightarrow{RREF}\left[\begin{array}{rrrrrr} 1 \amp  0 \amp  0 \amp  \frac{3}{2} \amp  \frac{3}{2} \amp  -\frac{3}{2} \\ 0 \amp  1 \amp  0 \amp  \frac{1}{2} \amp  \frac{9}{2} \amp  -\frac{3}{2} \\ 0 \amp  0 \amp  1 \amp  2 \amp  2 \amp  -1 \end{array} \right]</mrow>
        </md>
      </p>

      <p>
        Hence
        <me>
          [T]_\beta=\left[\begin{array}{rrr} \frac{3}{2} \amp  \frac{3}{2} \amp  -\frac{3}{2} \\ \frac{1}{2} \amp  \frac{9}{2} \amp  -\frac{3}{2} \\ 2 \amp  2 \amp  -1 \end{array} \right]
        </me>.
      </p>
    </statement>
  </example>

  <exercise xml:id="sumoflinearmaps">
    <statement>
      <p>
        Let <m>T,S\colon \R^n\to \R^m</m> be two linear maps.
        Then show that <m>T+S</m> is a linear map.
        Furthermore,
        the matrix of <m>T+S</m> is the sum of matrices of <m>T</m> and <m>S</m>.
      </p>
    </statement>
  </exercise>

  <p>
    Next we look the composition of linear maps.
  </p>
</subsection>

  <subsection xml:id="sec3-2-LT-composition" xmlns:xi="http://www.w3.org/2001/XInclude">
    <title>Composition of linear transformations</title>
    <p>
      Let <m>T\colon \R^n\to \R^m</m> and
      <m>S\colon R^m\to \R^p</m> be linear transformations.
      Then <m>S\circ T\colon \R^n\to \R^p</m> defined by <m>(S\circ T)(x)=S(T(x))</m> is a linear map.
    </p>

    <p>
      Suppose <m>T(x)=Ax</m> and <m>S(y)=By</m> are matrices transformations.
      Then
      <me>
        S(T(x))=S(Ax)=B(Ax)=(BA)x
      </me>.
      Thus the matrix of <m>S\circ T</m> is <m>BA</m>.
    </p>

    <example xml:id="linalg-engg-eg34">
      <statement>
        <p>
          Let <m>T\colon \R^4\to \R^3</m> and <m>S\colon \R^3\to \R^4</m> defined by
          <me>
            T\left(\begin{bmatrix}x_1\\x_2\\x_3\\x_4 \end{bmatrix} \right):= 
            \begin{bmatrix}x_{1} + x_{3} + x_{4} \\ x_{1} + x_{2} + 2  x_{3} - x_{4} \\ 2  x_{1} + x_{2} + 3  x_{3} - 2  x_{4} \end{bmatrix} 
          </me>
          and 
          <me>  
            S\left(\begin{bmatrix}y_1\\y_2\\y_3 \end{bmatrix} \right):= \begin{bmatrix}y_{1} + y_{3} \\ y_{1} + 3  y_{2} + 2  y_{3} \\ 2  y_{1} - y_{2} + 3  y_{3} \\ y_{2} - y_{3} \end{bmatrix}
          </me>
        </p>

        <p>
          Let <md><mrow>u_1=\left(1,-3,2,-1\right), u_2=\left(0,1,0,1\right)</mrow> 
            <mrow>u_3=\left(-1,2,-1,-1\right), u_4=\left(2,-8,4,-3\right)</mrow> 
            </md>  
          and define a basis
          <m>
            \beta = \left\{u_1,u_2,u_3,u_4\right\}
          </m>
          of <m>\R^4</m>. We take a basis
          <me>
            \gamma = \left\{v_1=\left(-1,1,1\right), v_2=\left(3,1,3\right), v_3=\left(2,-1,1\right)\right\}
          </me>
          of <m>\R^3</m>.
          Let <m>A=[T]_\beta^\gamma</m>,
          <m>B=[S]_\gamma^\beta</m> and <m>C=[S\circ T]_\beta^\beta</m>.
          Then we shall show that <m>C=BA</m>.
          Note that
          <me>
            S\circ T \left(\begin{bmatrix}x_1\\x_2\\x_3\\x_4 \end{bmatrix} \right) := \begin{bmatrix}3  x_{1} + x_{2} + 4  x_{3} - x_{4}\\ 8  x_{1} + 5  x_{2} + 13  x_{3} - 6  x_{4}\\ 7  x_{1} + 2  x_{2} + 9  x_{3} - 3  x_{4}\\ -x_{1} - x_{3} + x_{4} \end{bmatrix}
          </me>.
        </p>

        <p>
          First we find the matrix <m>A</m> using RREF
          <md>
            <mrow>\begin{bmatrix}v_1\amp  v_2 \amp  v_3 \amp  T(u_1) \amp  T(u_2) \amp  T(u_3)\amp  T(u_3) \end{bmatrix}  =\amp</mrow>
            <mrow>  \begin{bmatrix} -1 \amp  3 \amp  2 \amp  2 \amp  1 \amp  -3 \amp  3 \\ 
            1 \amp  1 \amp  -1 \amp  3 \amp  0 \amp  0 \amp  5 \\ 
            1 \amp  3 \amp  1 \amp  7 \amp  -1 \amp  -1 \amp  14 \end{bmatrix}\amp </mrow>
            <mrow> \xrightarrow{RREF}\begin{bmatrix} 1 \amp  0 \amp  0 \amp  3 \amp  -\frac{3}{2} \amp  \frac{7}{6} \amp  \frac{43}{6} \\ 
              0 \amp  1 \amp  0 \amp  1 \amp  \frac{1}{2} \amp  -\frac{5}{6} \amp  \frac{7}{6} \\ 
              0 \amp  0 \amp  1 \amp  1 \amp  -1 \amp  \frac{1}{3} \amp  \frac{10}{3} \end{bmatrix}\amp </mrow>
          </md>
        </p>

        <p>
          Hence <m>A = \left[\begin{array}{rrrr} 3 \amp  -\frac{3}{2} \amp  \frac{7}{6} \amp  \frac{43}{6} \\ 1 \amp  \frac{1}{2} \amp  -\frac{5}{6} \amp  \frac{7}{6} \\ 1 \amp  -1 \amp  \frac{1}{3} \amp  \frac{10}{3} \end{array} \right]</m>. 
          Next we find <m>B</m> using RREF
          <md>
            <mrow>\begin{bmatrix}u_1\amp u_2\amp u_3\amp u_4\amp S(v_1)\amp S(v_2)\amp S(v_3) \end{bmatrix}  =\amp</mrow> 
            <mrow>\begin{bmatrix} 1 \amp  0 \amp  -1 \amp  2 \amp  0 \amp  6 \amp  3 \\ 
            -3 \amp  1 \amp  2 \amp  -8 \amp  4 \amp  12 \amp  1 \\
            2 \amp  0 \amp  -1 \amp  4 \amp  0 \amp  14 \amp  8 \\ 
            -1 \amp  1 \amp  -1 \amp  -3 \amp  0 \amp  -2 \amp  -2 \end{bmatrix}\amp </mrow>
            <mrow>\xrightarrow{RREF}\begin{bmatrix} 1 \amp  0 \amp  0 \amp  0 \amp  8 \amp  56 \amp  19 \\ 
              0 \amp  1 \amp  0 \amp  0 \amp  -4 \amp  -16 \amp  -2 \\ 
              0 \amp  0 \amp  1 \amp  0 \amp  0 \amp  2 \amp  2 \\
              0 \amp  0 \amp  0 \amp  1 \amp  -4 \amp  -24 \amp  -7 \end{bmatrix}\amp</mrow>
          </md>
        </p>

        <p>
          Hence <m>B=\left[ \begin{array}{rrr} 8 \amp  56 \amp  19 \\ -4 \amp  -16 \amp  -2 \\ 0 \amp  2 \amp  2 \\ -4 \amp  -24 \amp  -7 \end{array} \right]</m>.
          It is easy to check that
          <me>BA= \left[\begin{array}{rrrr} 99 \amp -3 \amp -31 \amp 186 \\ 
            -30 \amp 0 \amp 8 \amp -54 \\ 
            4 \amp -1 \amp -1 \amp 9 \\ 
            -43 \amp 1 \amp 13 \amp -80 \end{array} \right]</me>.
          </p>

          <p>
            Now we find the matrix <m>C</m> of the composition <m>U=S\circ T</m> using RREF
          </p>
        
          <p>
          <md>
            <mrow>\begin{bmatrix}u_1\amp  u_2 \amp  u_3 \amp  u_4 \amp  U(u_1) \amp  U(u_2) \amp  U(u_3)\amp  U(u_4) \end{bmatrix}  =\amp </mrow>
            <mrow>\begin{bmatrix} 1 \amp  0 \amp  -1 \amp  2 \amp  9 \amp  0 \amp  -4 \amp  17 \\ 
              -3 \amp  1 \amp  2 \amp  -8 \amp  25 \amp  -1 \amp  -5 \amp  46 \\ 
              2 \amp  0 \amp  -1 \amp  4 \amp  22 \amp  -1 \amp  -9 \amp  43 \\ 
              -1 \amp  1 \amp  -1 \amp  -3 \amp  -4 \amp  1 \amp  1 \amp  -9 \end{bmatrix} \amp</mrow>
            <mrow>\xrightarrow{RREF}\begin{bmatrix} 1 \amp  0 \amp  0 \amp  0 \amp  99 \amp  -3 \amp  -31 \amp  186 \\ 
              0 \amp  1 \amp  0 \amp  0 \amp  -30 \amp  0 \amp  8 \amp  -54 \\ 
              0 \amp  0 \amp  1 \amp  0 \amp  4 \amp  -1 \amp  -1 \amp  9 \\ 
              0 \amp  0 \amp  0 \amp  1 \amp  -43 \amp  1 \amp  13 \amp  -80 \end{bmatrix}\amp </mrow>
          </md>
        </p>
        
        <p>
          This <m>C= \left[\begin{array}{rrrr} 99 \amp -3 \amp -31 \amp 186 \\ -30 \amp 0 \amp 8 \amp -54 \\ 4 \amp -1 \amp -1 \amp 9 \\ -43 \amp 1 \amp 13 \amp -80 \end{array} \right]</m>.
        </p>
        
        <p>
          Hence we have <m>C=BA</m>.
        </p>
      </statement>
    </example>
  </subsection>
 

  <subsection xml:id="sec3-2-LT-basis-change" xmlns:xi="http://www.w3.org/2001/XInclude">
    <title>Matrix of Change of basis</title>
    <p>
      Let <m>\beta=\{u_1,u_2\ldots,u_n\}</m> and
      <m>\gamma=\{v_1,v_2\ldots,v_n\}</m> be two bases of <m>\R^n</m>.
      Recall, the the definition of the matrix of change of bases <m>[I]_\beta^\gamma</m>.
      We obtained <m>[I]_\beta^\gamma</m> by applying RREF to the matrix <m>[B~|A]</m> and extracting the last <m>n</m> columns.
      This is nothing but the matrix of the identity linear map
      <m>I\colon \R^n\to \R^n</m> with respect to a basis <m>\beta</m> of the domain and <m>\gamma</m> of the codomain.
    </p>
    
    <p>
      Now let us consider what happens to the matrix of a linear transformation
      <m>T\colon \R^n\to \R^m</m> when we change the basis on domain and codoamin.
      Let <m>\beta=\{u_1,u_2\ldots,u_n\}</m> and
      <m>\gamma=\{v_1,v_2\ldots,v_m\}</m> be bases of <m>\R^n</m> and <m>\R^m</m> respectively.
      Let <m>A =[T]_\beta^\gamma</m> be the matrix of <m>T</m> with respect to <m>\beta</m> and <m>\gamma</m>.
      Let <m>\beta'=\{u_1',u_2'\ldots,u_n'\}</m> and
      <m>\gamma'=\{v_1',v_2'\ldots,v_m'\}</m> be another bases of <m>\R^n</m> and <m>\R^m</m> respectively.
      Let <m>B =[T]_{\beta'}^{\gamma'}</m> be the matrix of <m>T</m> with respect to <m>\beta'</m> and <m>\gamma'</m>.
      How are <m>A</m> and <m>B</m> related?
      The relation is given by the following commutative diagram.
    </p>

    <me>\begin{CD}
	(\R^n,\beta) @&gt;A=[T]_\beta^\gamma&gt;&gt; (\R^m,\gamma)\\
	@VV{\rho=[I]_\beta^{\beta'}}V @VV{\tau=[I]_\gamma^{\gamma'}}V\\
	(\R^n,\beta') @&gt;B=[T]_{\beta'}^{\gamma'}&gt;&gt;(\R^m,\gamma')
\end{CD}
    </me>
    
    <p>
      From the above commutative diagram, we have
      <me>
        \tau A = B\rho \implies B = \tau A \rho^{-1} \text{ or }  A = \tau^{-1}B\rho
      </me>.
    </p>
    
    <example xml:id="linalg-engg-eg35">
      <statement>
        <p>
          Consider a linear map <m>T\colon \R^4\to \R^3</m> defined in the <xref ref="linalg-engg-eg34">Example</xref>.
          Consider a basis<m>\beta=\{u_1,u_2,u_3,u_4\}</m> where
          <md>
          <mrow> u_1=\left(1,-3,2,-1\right),\amp  u_2=\left(0,1,0,1\right)</mrow> 
          <mrow> u_3=\left(-1,2,-1,-1\right),\amp  u_4=\left(2,-8,4,-3\right)</mrow>
          </md>
          of <m>\R^4</m> and a basis
          <me>
            \gamma = \left\{v_1=\left(-1,1,1\right), v_2=\left(3,1,3\right), v_3=\left(2,-1,1\right)\right\}
          </me>
          of <m>\R^3</m>.
          From <xref ref="linalg-engg-eg34">Example</xref>,
          <m>A=[T]_\beta^\gamma=\left[\begin{array}{rrrr} 3 \amp  -\frac{3}{2} \amp  \frac{7}{6} \amp  \frac{43}{6} \\ 1 \amp  \frac{1}{2} \amp  -\frac{5}{6} \amp  \frac{7}{6} \\ 1 \amp  -1 \amp  \frac{1}{3} \amp  \frac{10}{3} \end{array} \right]</m>.
          Let <m>\beta'=\{u_1',u_2',u_3',u_4'\}</m> where
          <md>
            <mrow>u_1'=\left(1,1,1,-1\right), \amp u_2'=\left(1,1,-1,1\right)</mrow>
            <mrow>u_3'=\left(1,-1,1,1\right), u_4'=\left(-1,1,1,1\right)</mrow>
          </md>
          be another basis of <m>\R^4</m>.
          
          Let
          <me>
            \gamma'=\{\left(0,1,1\right), \left(1,0,1\right), \left(1,1,0\right)\}
          </me>
          be another basis of <m>\R^3</m>.
          Then the matrix <m>B=[T]_{\beta'}^{\gamma'}=\left[\begin{array}{rrrr} 6 \amp  -2 \amp  0 \amp  0 \\ 2 \amp  0 \amp  2 \amp  0 \\ -1 \amp  1 \amp  1 \amp  1 \end{array} \right]</m>.
        </p>
   
        <p>
          The matrix of change of basis <m>\rho=[I]_\beta^\{\beta'\}=\left(\begin{array}{rrrr} \frac{1}{4} \amp 0 \amp \frac{1}{4} \amp \frac{1}{4} \\ -\frac{5}{4} \amp \frac{1}{2} \amp \frac{1}{4} \amp -\frac{13}{4} \\ \frac{5}{4} \amp 0 \amp -\frac{5}{4} \amp \frac{11}{4} \\ -\frac{3}{4} \amp \frac{1}{2} \amp \frac{1}{4} \amp -\frac{9}{4} \end{array} \right)</m>.
        </p>
   
        <p>
          The matrix of change of basis <m>\tau=[I]_\gamma^{\gamma'}=\left(\begin{array}{rrr} \frac{3}{2} \amp \frac{1}{2} \amp -1 \\ -\frac{1}{2} \amp \frac{5}{2} \amp 2 \\ -\frac{1}{2} \amp \frac{1}{2} \amp 0 \end{array} \right)</m>.
        </p>
   
        <p>
          It is easy to check that <m>B\rho = \tau A</m>.
        </p>
      </statement>
   
    </example>
   
    <p>
      Let <m>T\colon \R^n\to \R^n</m> be a linear transformation.
      Let <m>\beta=\{v_1,\ldots,
      v_n\}</m> be a basis of <m>\R^n</m> and <m>A=[T]_\beta</m>,
      the matrix of <m>T</m> with respect to <m>\beta</m>.
      Let <m>\gamma=\{u_1,\ldots,
      u_n\}</m> be another basis of <m>\R^n</m> and <m>B=[T]_\gamma</m>,
      the matrix of <m>T</m> with respect to <m>\gamma</m>.
      Let <m>\rho=[I]_\beta^{\gamma}</m> be matrix of change of basis from <m>\beta</m> to <m>\gamma</m>.
      Then we have <m>B = \rho^{-1}A\rho</m>.
      In this case,
      <m>A</m> and <m>B</m> are said to be similar matrices.
    </p>
   
    <definition xml:id="def-matrix-similarity">
      <statement>
        <p>
          Let <m>A</m> and <m>B</m> be two real <m>n\times n</m> matrices.
          Then <m>A</m> and <m>B</m> are called similar if there exists a non singular matrix <m>P</m> such that <m>B=P^{-1}AP</m>.
        </p>
      </statement>
    </definition>

    <remark xml:id="rem-defining-LT">
      <p>
        A linear transformation <m>T\colon \R^n\to \R^m</m> is completely determined once it is defined on a basis.
        In other words, Let <m>\beta=\{v_1,\ldots,
        v_n\}</m> be a basis of <m>\R^n</m>.
        Let <m>w_1,\ldots, w_n</m> be <m>n</m> vectors in <m>\R^m</m>.
        Then there exists a unique linear transformation <m>T\colon \R^n\to \R^m</m> such that
        <m>T(v_i)=w_i</m> for <m>i=1,\ldots, n</m>.
      </p>
    </remark>
    
    <p>
      How is <m>T</m> defined, if <m>T(v_i)=w_i</m>?
      For <m>v\in V</m>, there exist scalars,
      <m>\alpha_1,\ldots, \alpha_n</m> such that <m>v=\sum \alpha_iv_i</m>.
      Then <m>T(v)=\sum \alpha T(v_1)=\sum\alpha w_i</m>.
    </p>
    
    <reading-questions xml:id="rqs-uniqueness-of-LT">
      <p>
        Prove the uniqueness of the linear tranformation in the <xref ref="rem-defining-LT"/>
      </p>
    </reading-questions>

    <example xml:id="linalg-engg-eg40">
      <statement>
        <p>
          Fix a basis <m>\beta =\{ (1,1,-1),(1,-1,1),(-1,1,1)\}</m> of <m>\R^3</m>.
          Define a linear map <m>T\colon \R^3\to \R^3</m> such that <m>T(1,1,-1)=(1,1,0), T(1,-1,1)=(1,0,1), T(-1,1,1)=(0,1,1)</m>.
          Find <m>T\left(\begin{bmatrix}x_1\\ x_2\\ x_3 \end{bmatrix} \right)</m>.
        </p>
        <p>
          We have
          <me>
            T\left(\begin{bmatrix}x_1\\ x_2\\ x_3 \end{bmatrix} \right)=T(x_1e_1+x_2e_2+x_3e_3)=x_1T(e_1)+x_2T(e_2)+x_3T(e_3)
          </me>.
        </p>
        
        <p>
          Thus in order to find <m>T</m> we need to know how is <m>T</m> defined on the standard basis vector.
          First we need to find the coordinates of
          <m>e_1,e_2,e_2</m> with respect to the basis <m>\beta</m> using RREF.
          <md>
            <mrow>\begin{bmatrix}v_1 \amp  v_2 \amp  v_3 \amp | \amp  e_1 \amp  e_2 \amp  e_3 \end{bmatrix} = \amp
              \left[\begin{array}{rrr|rrr} 1 \amp  1 \amp  -1 \amp  1 \amp  0 \amp  0 \\ 
              1 \amp  -1 \amp  1 \amp  0 \amp  1 \amp  0 \\ 
              -1 \amp  1 \amp  1 \amp  0 \amp  0 \amp  1 \end{array} \right]</mrow> 
            <mrow>\amp  \xrightarrow{RREF} 
              \left[\begin{array}{rrr|rrr} 1 \amp  0 \amp  0 \amp  \frac{1}{2} \amp  \frac{1}{2} \amp  0 \\ 
              0 \amp  1 \amp  0 \amp  \frac{1}{2} \amp  0 \amp  \frac{1}{2} \\ 
              0 \amp  0 \amp  1 \amp  0 \amp  \frac{1}{2} \amp  \frac{1}{2} \end{array} \right]</mrow>
          </md>.
        </p>
        
        <p>
          We have
          <me>
            \begin{aligned} e_1 = 1/2 v_1+1/2v_2 \implies   T(e_1)=1/2 w_1+1/2 w_2=(1, 1/2, 1/2).\\ 
            e_2 = 1/2 v_1+1/2v_3 \implies   T(e_2)=1/2 w_1+1/2 w_3=(1/2, 1, 1/2).\\ 
            e_3 = 1/2 v_2+1/2v_3 \implies T(e_3)=1/2 w_2+1/2 w_3=(1/2, 1/2, 1). \end{aligned}
          </me>
          <md>
            <mrow>T\left(\begin{bmatrix}x_1\\ x_2\\ x_3 \end{bmatrix} \right) =\amp x_1T(e_1)+x_2T(e_2)+x_3T(e_3)</mrow>
            <mrow> =\amp x_1(1, 1/2, 1/2)+x_2(1/2, 1, 1/2)+x_3(1/2, 1/2, 1)</mrow>
            <mrow>=\amp  \begin{bmatrix}x_{1} + \frac{1}{2}  x_{2} + \frac{1}{2}  x_{3}\\ 
              \frac{1}{2}  x_{1} + x_{2} + \frac{1}{2}  x_{3}\\ 
              \frac{1}{2}  x_{1} + \frac{1}{2}  x_{2} + x_{3} \end{bmatrix} </mrow>
          </md>.
        </p>
        
        <p>
          It is easy to check that <m>T(v_i)=w_i</m>.
        </p>
      </statement>
    </example>
 
 
   </subsection>
  </section>
