<?xml version="1.0" encoding="UTF-8"?>

<section xml:id="sec6-1-GramSchmidt" xmlns:xi="http://www.w3.org/2001/XInclude">
  <title>Gram-Schmidt Orthogonalization Process</title>

  
    <p>
     In this section, we look at how to construct an 
     orthogonal basis of <m>\R^n</m> from a basis. 
    </p>
 
  <p>
    Let <m>\{v_1,\ldots, v_n\}</m> be a basis of <m>\R^n</m>.
    Define
    <md>
      <mrow>u_1:  =\amp  v_1</mrow>
      <mrow>u_2:  =\amp  v_2 -\frac{u_2\cdot u_1}{\norm{u_1}^2}u_1</mrow>
      <mrow>u_3:  =\amp  v_3 -\frac{v_3\cdot u_1}{\norm{u_1}^2}u_1-\frac{v_3\cdot u_2}{\norm{u_2}^2}u_2</mrow>
      <mrow> \amp  \vdots</mrow>
      <mrow>u_n:  =\amp  v_n -\frac{v_n\cdot u_1}{\norm{u_1}^2}u_1-\cdots -\frac{v_n\cdot u_{n-1}}{\norm{u_{n-1}}^2}u_{n-1}</mrow>
    </md>
  </p>
  <p>
    In view of Ex.
    <xref ref="orth-ex2-1"></xref>,
    it is easy to see that <m>\{u_1,\ldots,
    u_n\}</m> is an orthogonal basis of <m>\R^n</m>.
    Now we normalize <m>u_i's</m>.
    Define <m>q_i=\frac{u_i}{\norm{u_i}}</m>.
    Then <m>\{q_1,\cdots, q_n\}</m> is an orthononal basis of <m>\R^n</m>.
    Note that we could have defined <m>q_i</m> immediately after defining <m>u_i</m>.
  </p>
  <p>
    This process is called the <em>Gram-Schmidt orthogonalization process</em>.
  </p>

  <p>
    Geometrically <m>u_2</m>,
    constructed by subtracting the orthogonal projection of <m>v_2</m> on to <m>u_1</m>.
    In order to construct <m>u_3</m>,
    we take sum of orthogonal projections of <m>v_3</m> onto <m>u_1</m> and <m>u_2</m>,
    which is the orthogonal projection of the plane spanned by <m>u_1</m> and <m>u_2</m> and subtract this from <m>v_3</m>.
    Readers are encouraged to draw figures.
  </p>

  <example xml:id="gram-schmidt-eg1">
    <statement>
      <p>
        Use the Gram-Schmidt orthogonalization process to find an orthonormal basis of <m>\R^3</m> starting with a basis <m>\{(0,1,1), (1,1,1), (1,-2,2)\}</m>.
        Let <m>v_1 = (0, 1, 1), v_2=(1, 1, 1), v_3=(1, -2, 2)</m>.
        Then we have
        <md>
          <mrow>u_1: = \amp (0, 1, 1)</mrow>
          <mrow>u_2:  = \amp v_2 -\frac{u_2\cdot u_1}{\norm{u_1}^2}u_1=(1, 1, 1)-\frac{2}{2}(0,1,1)=(1,0,0)</mrow>
          <mrow>u_3:= \amp v_3 -\frac{u_3\cdot u_1}{\norm{u_1}^2}u_1-\frac{u_3\cdot u_2}{\norm{u_2}^2}u_2</mrow>
          <mrow> =  \amp (1, -2, 2)-\frac{0}{2}(0,1,1)-\frac{1}{1}(1,0,0)=(0,-2,2)</mrow>
        </md>
      </p>

      <p>
        Thus the orthonormal basis obtained from the given basis is
        <me>
          \left\{q_1 = \left(0, \frac{1}{\sqrt{2}}, \frac{1}{\sqrt{2}}\right), q_2=(1,0,0), q_3 =\left(0,\frac{-1}{\sqrt{2}},\frac{1}{\sqrt{2}}\right)\right\}
        </me>.
      </p>
    </statement>
  </example>

  <example xml:id="gram-schmidt-eg2">
    <statement>
      <p>
        Consider the matrix <m>A=\left(\begin{array}{rrrr} -1 \amp 1 \amp 0 \amp 1 \\ 1 \amp -1 \amp 0 \amp 1 \\ -1 \amp 0 \amp 2 \amp 1 \end{array} \right)</m>.
        Find an orthogonal basis of the row space of <m>A</m>.
        It is easy to check that rank of <m>A</m> is 3.
        Hence row are linearly independent vectors in <m>\R^4</m>.
      </p>

      <p>
        Let
        <m>
          v_1=(-1,1,0,1), v_2 = (1,-1,0,1),   v_3=(-1,0,2,1)
        </m>.
        <md><mrow>u_1: = \amp (-1,1,0,1)</mrow>
          <mrow>u_2: =  \amp v_2 -\frac{u_2\cdot u_1}{\norm{u_1}^2}u_1</mrow>
           <mrow> =\amp (1,-1,0,1)-\frac{-1}{3}(-1,1,0,1)=(2/3, -2/3, 0, 4/3)</mrow>
          <mrow>u_3: = \amp  v_3 -\frac{u_3\cdot u_1}{\norm{u_1}^2}u_1-\frac{u_3\cdot u_2}{\norm{u_2}^2}u_2</mrow>
          <mrow>  = \amp  (-1,0,2,1)-\frac{2}{3}(-1,1,0,1)-\frac{2/3}{9/2}(2/3, -2/3, 0, 4/3)</mrow>
          <mrow>=\amp (-1/2, -1/2, 2, 0)
          </mrow>
        </md>
      </p>

      <p>
        Hence
        <me>
          \{(-1, 1, 0, 1) (2/3, -2/3, 0, 4/3) (-1/2, -1/2, 2, 0)\}
        </me>
        is an orthogonal basis of the row space of <m>A</m>.
      </p>
    </statement>
  </example>

  <exercise>
    <statement>
      <p>
        Use the Gram-Schmidt orthogonalization process to find an orthonormal basis of <m>\R^3</m> starting with a basis <m>\beta=\{(1,1,1),(-1,1,1),(-1,0,1)\}</m>.
      </p>
    </statement>
  </exercise>
  
  <exercise>
    <statement>
      <p>
        Use the Gram-Schmidt orthogonalization process to find an orthonormal basis of the subspace <m>W\subset \R^4</m> with basis
        <me>
          \beta = \{ (-1,1,1,0),(-1,0,1,0),(1,0,0,1)\}
        </me>.
      </p>
    </statement>
  </exercise>
  
</section>
